move parser/serializer spec combinators to CDDL.Spec.*

share/pulse/examples/dice/cbor/CDDL.Spec.ArrayGroup.fst
@@ -545,7 +545,7 @@ let array_group3_concat_unique_weak_zero_or_more_right
   ))
 = ()
 
-#push-options "--z3rlimit 16"
+#push-options "--z3rlimit 32"
 #restart-solver
 
 let array_group3_concat_unique_weak_zero_or_more'
@@ -780,4 +780,33 @@ let array_group3_concat_close
     (close_array_group (array_group3_concat a1 a2))
     (array_group3_concat a1 (close_array_group a2))
   )
+= ()
+
+#push-options "--z3rlimit 16"
+#restart-solver
+let array_group_parser_spec_concat
+  (#source1: array_group3 None)
+  (#target1: Type)
+  (#target_size1: target1 -> nat)
+  (p1: array_group_parser_spec source1 target_size1)
+  (#source2: array_group3 None)
+  (#target2: Type)
+  (#target_size2: target2 -> nat)
+  (p2: array_group_parser_spec source2 target_size2 {
+    array_group3_concat_unique_weak source1 source2
+  })
+  (target_size: (target1 & target2) -> nat {
+    forall x . target_size x == target_size1 (fst x) + target_size2 (snd x)
+  })
+: Tot (array_group_parser_spec (array_group3_concat source1 source2) target_size)
+= fun x ->
+  let Some (x1, x2) = source1 x in
+  assert (source1 x1 == Some (x1, []));
+  List.Tot.append_length x1 x2;
+  (p1 x1, p2 x2)
+
+#pop-options
+
+let array_group_parser_spec_concat_eq
+  p1 p2 target_size x
 = ()
