share/pulse/examples/dice/cbor/CDDL.Spec.Misc.fst
@@ -89,3 +89,23 @@ let bstr_cbor
     Cbor.data_item_wf data_item_order y /\
     ty y == true
   )
+
+let parser_spec_bool : parser_spec t_bool bool =
+  (fun x -> let Cbor.Simple v = x in
+    v = simple_value_true
+  )
+
+let serializer_spec_bool : serializer_spec parser_spec_bool =
+  (fun x -> Cbor.Simple (if x then simple_value_true else simple_value_false))
+
+let parser_spec_bstr : parser_spec bstr string64 =
+  (fun x -> let Cbor.String _ v = x in v)
+
+let serializer_spec_bstr : serializer_spec parser_spec_bstr =
+  (fun x -> Cbor.String Cbor.cbor_major_type_byte_string x)
+
+let parser_spec_tstr : parser_spec tstr string64 =
+  (fun x -> let Cbor.String _ v = x in v)
+
+let serializer_spec_tstr : serializer_spec parser_spec_tstr =
+  (fun x -> Cbor.String Cbor.cbor_major_type_text_string x)
